# HW11
## 6.3Exercise

### 21
21. How many permutations of the letters ABCDEFG contain 
- a) the string BCD? 
- b) the string CFGA? 
- c) the strings BA and GF? 
- d) the strings ABC and DE? 
- e) the strings ABC and CDE? 
- f ) the strings CBA and BED?

### answer
- a) $5! = 120$
- b) $4! = 24$
- c) $5! = 120$
- d) $4! = 24$
- e) $3! = 6$
- f ) $0$
---

### 31

∗ 31. How many 4-permutations of the positive integers not exceeding 100 contain three consecutive integers $k$, $k + 1$, $k + 2$, in the correct order 
- a) where these consecutive integers can perhaps be separated by other integers in the permutation? 
- b) where they are in consecutive positions in the permutation?

### answer
- a) We need to select 4 numbers, including three consecutive integers k, k+1, k+2 (in the correct order).

First, we need to choose the value of k. Since we're selecting from positive integers not exceeding 100, and we need k, k+1, k+2 to be in range, k can be from 1 to 98, giving us 98 possibilities.

Next, we need to select the fourth number. This number can't be k, k+1, or k+2, so we choose 1 number from the remaining 97 numbers, giving 97 possibilities.

Finally, we need to arrange these 4 numbers so that k, k+1, k+2 appear in the correct order. This means we first determine the positions for k, k+1, k+2, then place the fourth number.

There are $\binom{4}{3} = 4$ ways to choose positions for k, k+1, k+2, with their internal order fixed. The fourth number goes in the remaining position.

Therefore, the total number of permutations is: $98 \times 97 \times 4 = 38024$

- b) In this case, k, k+1, k+2 must appear consecutively in the permutation.

First, we still need to choose the value of k, which ranges from 1 to 98, giving 98 possibilities.

Next, we select the fourth number from the remaining 97 numbers, giving 97 possibilities.

Then, we can treat k, k+1, k+2 as a single unit and arrange it with the fourth number. This is equivalent to arranging 2 elements, which can be done in $2! = 2$ ways.

Therefore, the total number of permutations is: $98 \times 97 \times 2 = 19012$

---

### 38
38. How many bit strings contain exactly five 0s and 14 1s if every 0 must be immediately followed by two 1s?

### answer
So we have five $011$ bit strings and four free $1$ bit string.
Use the binomial theorem,
there are $\binom{9}{4}=126$ bit strings. 

---

## 6.4Exercise
### 7
7. What is the coefficient of $x^9$ in $(2 - x)^{19}$?

### answer
Using the binomial theorem, the expansion of $x^9$ in $(2 - x)^{19}$ is
$(2 - x)^{19} = \sum_{k=0}^{19} \binom{19}{k} (2)^{19-k} (-x)^k$
For $x^9$, $k = 9$.
$\binom{19}{9} = 92378$
$\binom{19}{9}*2^{10}*(-1)^9 = -94595072$
the coefficient is $-94595072$

---

### 13
13. Use the binomial theorem to find the coefficient of $x^ay^b$ in the expansion of $(2x^3 - 4y^2)^7$, where  
- a) $a = 9$, $b = 8$. 
- b) $a = 8$, $b = 9$. 
- c) $a = 0$, $b = 14$. 
- d) $a = 12$, $b = 6$. 
- e) $a = 18$, $b = 2$.

### answer
Using the binomial theorem, the expansion of $(2x^3 - 4y^2)^7$ is:
$(2x^3 - 4y^2)^7 = \sum_{k=0}^{7} \binom{7}{k} (2x^3)^{7-k} (-4y^2)^k$

- a) $a = 9$, $b = 8$:
   For $x^9$, $k = 4$.
   For $y^8$, $k = 4$.
   The coefficient is $\binom{7}{4} \cdot 2^3 \cdot (-4)^4 = 35 \cdot 8 \cdot 256 = 71680$

- b) $a = 8$, $b = 9$:
   No solution exists because if $3(7-k) = 8$, then $7-k = 8/3$, which is not an integer.
   Therefore, the coefficient is 0.

- c) $a = 0$, $b = 14$:
   For $x^0$, $k = 7$.
   For $y^{14}$, $k = 7$.
   The coefficient is $\binom{7}{7} \cdot 2^0 \cdot (-4)^7 = 1 \cdot 1 \cdot (-4)^7 = -16384$

- d) $a = 12$, $b = 6$:
   For $x^{12}$, $k = 3$.
   For $y^6$, $k = 3$.
   The coefficient is $\binom{7}{3} \cdot 2^4 \cdot (-4)^3 = 35 \cdot 16 \cdot (-64) = -35840$

- e) $a = 18$, $b = 2$:
   For $x^{18}$, $k = 1$.
   For $y^2$, $k = 1$.
   The coefficient is $\binom{7}{1} \cdot 2^6 \cdot (-4)^1 = 7 \cdot 64 \cdot (-4) = -1792$

---

### 27
27. Show that if $n$ and $k$ are positive integers, then $\binom{n+1}{k} = \frac{(n+1)\binom{n}{k-1}}{k}$. Use this identity to construct an inductive definition of the binomial coefficients.

### answer
We need to prove that $\binom{n+1}{k} = \frac{(n+1)\binom{n}{k-1}}{k}$ for positive integers $n$ and $k$.

Starting with the definition of binomial coefficients:
$\binom{n+1}{k} = \frac{(n+1)!}{k!(n+1-k)!}$

We can rewrite this as:
$\binom{n+1}{k} = \frac{(n+1)!}{k!(n+1-k)!} = \frac{(n+1) \cdot n!}{k \cdot (k-1)! \cdot (n+1-k)!}$

Now, we can recognize that $\binom{n}{k-1} = \frac{n!}{(k-1)!(n-(k-1))!} = \frac{n!}{(k-1)!(n-k+1)!}$

Substituting this into our expression:
$\binom{n+1}{k} = \frac{(n+1) \cdot n!}{k \cdot (k-1)! \cdot (n+1-k)!} = \frac{(n+1)}{k} \cdot \frac{n!}{(k-1)!(n-k+1)!} = \frac{(n+1)\binom{n}{k-1}}{k}$

Therefore, $\binom{n+1}{k} = \frac{(n+1)\binom{n}{k-1}}{k}$ is proven.

Using this identity, we can construct an inductive definition of binomial coefficients:

**Base cases:**
- $\binom{n}{0} = 1$ for all $n \geq 0$
- $\binom{n}{n} = 1$ for all $n \geq 0$

**Inductive step:**
- For $1 \leq k \leq n$, $\binom{n+1}{k} = \frac{(n+1)\binom{n}{k-1}}{k}$


---

### 31
∗ 31. Prove the hockeystick identity $\sum_{k=0}^{r} \binom{n+k}{k} = \binom{n+r+1}{r}$ whenever $n$ and $r$ are positive integers, 
- a) using a combinatorial argument. 
- b) using Pascal's identity.

### answer
- a) Combinatorial Proof:
Pf:
Consider selecting r people from a group of n+r+1 people. By definition, there are $\binom{n+r+1}{r}$ ways to do this.
Alternatively, we can classify the selection based on the position of the last person selected:
  - If the last person selected is in position n+0, then we need to select r-0 people from the first n-1+0 people, giving $\binom{n-1}{r}$ ways
  - If the last person selected is in position n+1, then we need to select r-1 people from the first n-1+1 people, giving $\binom{n}{r-1}$ ways
  - If the last person selected is in position n+2, then we need to select r-1 people from the first n-1+2 people, giving $\binom{n+1}{r-1}$ ways
  - ...
  - If the last person selected is in position n+r, then we need to select r-1 people from the first n-1+r people, giving $\binom{n+r-1}{r-1}$ ways

  By reindexing, these cases can be represented as $\sum_{k=0}^{r} \binom{n+k-1}{r-1}$. Using the combinatorial identity $\binom{n+k-1}{r-1} = \binom{n+k}{k}$, we get $\sum_{k=0}^{r} \binom{n+k}{k} = \binom{n+r+1}{r}$.
  Q.E.D

- b) Proof using Pascal's identity:
Pf: By induction
**Base case:**
For $r=1$:
$\sum_{k=0}^{1} \binom{n+k}{k} = \binom{n}{0} + \binom{n+1}{1} = 1 + (n+1) = n+2 = \binom{n+1+1}{1}$, which is true.
**Inductive Step:**
Assume that for some r ≥ 1, $\sum_{k=0}^{r} \binom{n+k}{k} = \binom{n+r+1}{r}$ holds.
For r+1, we have:
$\sum_{k=0}^{r+1} \binom{n+k}{k} = \sum_{k=0}^{r} \binom{n+k}{k} + \binom{n+r+1}{r+1}$
By our induction hypothesis, $\sum_{k=0}^{r} \binom{n+k}{k} = \binom{n+r+1}{r}$
So $\sum_{k=0}^{r+1} \binom{n+k}{k} = \binom{n+r+1}{r} + \binom{n+r+1}{r+1}$
Using Pascal's identity $\binom{n+r+1}{r} + \binom{n+r+1}{r+1} = \binom{n+r+2}{r+1}$
Therefore $\sum_{k=0}^{r+1} \binom{n+k}{k} = \binom{n+r+2}{r+1}$, which matches our formula.
Q.E.D

---

## 6.5Exercise
### 15
15. How many solutions are there to the equation  $x_1 + x_2 + x_3 + x_4 + x_5 = 21$,  where $x_i$, $i = 1, 2, 3, 4, 5$, is a nonnegative integer such that  
- a) $x_1 \geq 1$? 
- b) $x_i \geq 2$ for $i = 1, 2, 3, 4, 5$? 
- c) $0 \leq x_1 \leq 10$? 
- d) $0 \leq x_1 \leq 3$, $1 \leq x_2 < 4$, and $x_3 \geq 15$?

### answer
Just consider to tuck $4$ columns into 22 slots, collision is allowed. And $a_i$ is the quantity of gap from the previous column.
- a) $\binom{20 + 5 - 1}{5 - 1} = \binom{24}{4}$
- b) $\binom{15}{4} = 1365$
- c) $\sum_{k=0}^{10} \binom{24-k}{3}$
- d) $x_3'=x_3-15$, $x_1+x_2+x_3'+x_4+x_5 = 6$
- 
| $x_1$ | $x_2$ | $6-x_1-x_2$ | $\binom{\text{remained}+3-1}{3-1}$ |
|-------|-------|-------------------|---------------------------|
| 0     | 1     | 5                 | $\binom{7}{2}=21$         |
| 0     | 2     | 4                 | $\binom{6}{2}=15$         |
| 0     | 3     | 3                 | $\binom{5}{2}=10$         |
| 1     | 1     | 4                 | $\binom{6}{2}=15$         |
| 1     | 2     | 3                 | $\binom{5}{2}=10$         |
| 1     | 3     | 2                 | $\binom{4}{2}=6$          |
| 2     | 1     | 3                 | $\binom{5}{2}=10$         |
| 2     | 2     | 2                 | $\binom{4}{2}=6$          |
| 2     | 3     | 1                 | $\binom{3}{2}=3$          |
| 3     | 1     | 2                 | $\binom{4}{2}=6$          |
| 3     | 2     | 1                 | $\binom{3}{2}=3$          |
| 3     | 3     | 0                 | $\binom{2}{2}=1$          |

so the answer is $106$

---

### 21
21. A Swedish tour guide has devised a clever way for his clients to recognize him. He owns 13 pairs of shoes of the same style, customized so that each pair has a unique color. How many ways are there for him to choose a left shoe and a right shoe from these 13 pairs 
- a) without restrictions and which color is on which foot matters? 
- b) so that the colors of the left and right shoe are different and which color is on which foot matters? 
- c) so that the colors of the left and right shoe are different but which color is on which foot does not matter? 
- d) without restrictions, but which color is on which foot does not matter?

### answer

- a) $13*13=169$
- b) $13*12=156$
- c) $\binom{13}{2} = 78$
- d) $13 + 78 = 91$
---

### 42
42. How many ways are there to travel in $xyzw$ space from the origin $(0, 0, 0, 0)$ to the point $(4, 3, 5, 4)$ by taking steps one unit in the positive $x$, positive $y$, positive $z$, or positive $w$ direction?

### answer
Consider there are 4 $x$ steps, 3 $y$ steps, 5 $z$ steps and 4 $w$ steps, and we need to compose these steps.
So there is $\frac{16!}{3!4!4!5!} = 50450400$

---

## 8.1Exercise
### 7
7. 
- a) Find a recurrence relation for the number of bit strings of length n that contain a pair of consecutive 0s. 
- b) What are the initial conditions? 
- c) How many bit strings of length seven contain two consecutive 0s?

### answer
- a) If the $n$ length bit string 
  - start with $1$: then there is $a_{n-1}$ possibilities.
  - start with $00$: then there is $2^{n-2}$ possibilities.
  - start with $01$: then there is $a_{n-2}$ possibilities.
 
  so the answer is $a_{n-1} + a_{n-2} + 2^{n-2}$
- b) $a_0 = 0$, $a_1 = 0$, $a_2 = 1$
- c) $94$
---

### 17
∗ 17. 
- a) Find a recurrence relation for the number of ternary strings of length n that do not contain consecutive symbols that are the same. 
- b) What are the initial conditions? 
- c) How many ternary strings of length six do not contain consecutive symbols that are the same?

### answer
- a) Consider a $n$ length string, by symmetry, we know that the quantity of the target string start with $0$ is equal to the quantity start with $1$ and $2$. So for the $n+1$ length, we just need to make the last number be different with the previous.
So $a_{n+1} = 2 * a_n$
- b) $a_0 = 1, \quad a_1 = 3$
- c) $96$

---

### 26
26. 
- a) Find a recurrence relation for the number of ways to completely cover a 2 × n checkerboard with 1 × 2 dominoes. [Hint: Consider separately the coverings where the position in the top right corner of the checkerboard is covered by a domino positioned horizontally and where it is covered by a domino positioned vertically.] 
- b) What are the initial conditions for the recurrence relation in part (a)? 
- c) How many ways are there to completely cover a 2 × 17 checkerboard with 1 × 2 dominoes?

### answer

- a) Consider the right up corner. that domino is:
  - **horizon**: then there is $a_n-2$ possibility.
  - **vertical**:then there is $a_n-1$ possibility.

  so $a_n = a_{n-1} + a_{n-2}$

- b) $a_1 = 1 \quad a_2 = 2$
- c) $2584$

---

### 48
Let $\{a_n\}$ be a sequence of real numbers. The backward differences of this sequence are defined recursively as shown next. The first difference $\nabla a_n$ is  $\nabla a_n = a_n - a_{n-1}$.  The $(k + 1)$st difference $\nabla^{k+1}a_n$ is obtained from $\nabla^k a_n$ by  $\nabla^{k+1}a_n = \nabla^k a_n - \nabla^k a_{n-1}$.

48. Show that $a_{n-1} = a_n - \nabla a_n$.

### answer

we know $\nabla a_n$ is  $\nabla a_n = a_n - a_{n-1}$.
So $a_{n-1} = a_n - \nabla a_n$

---